Hacl.Conversions: starting cleanup

crypto_hst/utils/Hacl.Conversions.fst
@@ -12,68 +12,118 @@ open Hacl.UInt32
 open Hacl.SBuffer
 open Hacl.Operations
 
+
+module U8 = FStar.UInt8
+module S8 = Hacl.UInt8
+module U32 = FStar.UInt32
+module S32 = Hacl.UInt32
+module U64 = FStar.UInt64
+module S64 = Hacl.UInt64
+
+let u8 = FStar.UInt8.t
+let s8 = Hacl.UInt8.t
 let u32 = FStar.UInt32.t
+let s32 = Hacl.UInt32.t
 let u64 = FStar.UInt64.t
 let s64 = Hacl.UInt64.t
-let s32 = Hacl.UInt32.t
-let s8 = Hacl.UInt8.t
 let uint32s = Hacl.SBuffer.u32s
 let bytes = Hacl.SBuffer.u8s
+
+
+
+//
+// All this **** is required because the way those things
+// are formalized in Hacl is wrong. It should disappear when
+// we change the representation of buffers in the F* stdlib.
+//
+
+val be_bytes_of_sint64: b:bytes{length b >= 8} -> x:s64
+  -> STL unit
+        (requires (fun h -> live h b))
+        (ensures (fun h0 _ h1 -> live h1 b /\ modifies_1 b h0 h1))
+
+let be_bytes_of_sint64 output x =
+ let b0 = sint64_to_sint8 (S64.logand (S64.shift_right x 56ul) (uint32_to_sint64 255ul)) in
+ let b1 = sint64_to_sint8 (S64.logand (S64.shift_right x 48ul) (uint32_to_sint64 255ul)) in
+ let b2 = sint64_to_sint8 (S64.logand (S64.shift_right x 40ul) (uint32_to_sint64 255ul)) in
+ let b3 = sint64_to_sint8 (S64.logand (S64.shift_right x 32ul) (uint32_to_sint64 255ul)) in
+ let b4 = sint64_to_sint8 (S64.logand (S64.shift_right x 24ul) (uint32_to_sint64 255ul)) in
+ let b5 = sint64_to_sint8 (S64.logand (S64.shift_right x 16ul) (uint32_to_sint64 255ul)) in
+ let b6 = sint64_to_sint8 (S64.logand (S64.shift_right x 8ul)  (uint32_to_sint64 255ul)) in
+ let b7 = sint64_to_sint8 (S64.logand x (uint32_to_sint64 255ul)) in
+ upd output 0ul b0;
+ upd output 1ul b1;
+ upd output 2ul b2;
+ upd output 3ul b3;
+ upd output 4ul b4;
+ upd output 5ul b5;
+ upd output 6ul b6;
+ upd output 7ul b7
+
+
+val be_bytes_of_uint64: b:bytes{length b >= 8} -> x:u64
+  -> STL unit
+        (requires (fun h -> live h b))
+        (ensures (fun h0 _ h1 -> live h1 b /\ modifies_1 b h0 h1))
+
+let be_bytes_of_uint64 output x =
+ let b0 = sint64_to_sint8 (S64.logand (uint64_to_sint64 (U64.shift_right x 56ul)) (uint32_to_sint64 255ul)) in
+ let b1 = sint64_to_sint8 (S64.logand (uint64_to_sint64 (U64.shift_right x 48ul)) (uint32_to_sint64 255ul)) in
+ let b2 = sint64_to_sint8 (S64.logand (uint64_to_sint64 (U64.shift_right x 40ul)) (uint32_to_sint64 255ul)) in
+ let b3 = sint64_to_sint8 (S64.logand (uint64_to_sint64 (U64.shift_right x 32ul)) (uint32_to_sint64 255ul)) in
+ let b4 = sint64_to_sint8 (S64.logand (uint64_to_sint64 (U64.shift_right x 24ul)) (uint32_to_sint64 255ul)) in
+ let b5 = sint64_to_sint8 (S64.logand (uint64_to_sint64 (U64.shift_right x 16ul)) (uint32_to_sint64 255ul)) in
+ let b6 = sint64_to_sint8 (S64.logand (uint64_to_sint64 (U64.shift_right x 8ul))  (uint32_to_sint64 255ul)) in
+ let b7 = sint64_to_sint8 (S64.logand (uint64_to_sint64 x) (uint32_to_sint64 255ul)) in
+ upd output 0ul b0;
+ upd output 1ul b1;
+ upd output 2ul b2;
+ upd output 3ul b3;
+ upd output 4ul b4;
+ upd output 5ul b5;
+ upd output 6ul b6;
+ upd output 7ul b7
+
+
+val be_bytes_of_sint32: b:bytes{length b >= 4} -> x:s32
+  -> STL unit
+        (requires (fun h -> live h b))
+        (ensures (fun h0 _ h1 -> live h1 b /\ modifies_1 b h0 h1))
+
+let be_bytes_of_sint32 output x =
+ let b0 = sint32_to_sint8 (S32.logand (S32.shift_right x 24ul) (uint32_to_sint32 255ul)) in
+ let b1 = sint32_to_sint8 (S32.logand (S32.shift_right x 16ul) (uint32_to_sint32 255ul)) in
+ let b2 = sint32_to_sint8 (S32.logand (S32.shift_right x 8ul)  (uint32_to_sint32 255ul)) in
+ let b3 = sint32_to_sint8 (S32.logand x (uint32_to_sint32 255ul)) in
+ upd output 0ul b0;
+ upd output 1ul b1;
+ upd output 2ul b2;
+ upd output 3ul b3
+
+
+val be_bytes_of_uint32: b:bytes{length b >= 4} -> y:u32
+  -> STL unit
+        (requires (fun h -> live h b))
+        (ensures (fun h0 _ h1 -> live h1 b /\ modifies_1 b h0 h1))
+
+let be_bytes_of_uint32 output x =
+ let b0 = uint32_to_sint8 (U32.logand (U32.shift_right x 24ul) 255ul) in
+ let b1 = uint32_to_sint8 (U32.logand (U32.shift_right x 16ul) 255ul) in
+ let b2 = uint32_to_sint8 (U32.logand (U32.shift_right x 8ul)  255ul) in
+ let b3 = uint32_to_sint8 (U32.logand x 255ul) in
+ upd output 0ul b0;
+ upd output 1ul b1;
+ upd output 2ul b2;
+ upd output 3ul b3
 
 
 #set-options "--lax"
 
 
-let op_At_Amp (a:s64) (s:s64) : Tot s64 = Hacl.UInt64.logand a s
-
-val be_bytes_of_sint64: x:bytes -> y:s64
-  -> STL unit (requires (fun h -> live h x)) (ensures (fun h0 _ h1 -> live h1 x /\ modifies_1 x h0 h1))
-let be_bytes_of_sint64 output x =
- let b0 = sint64_to_sint8 ((Hacl.UInt64.shift_right x 56ul) @& uint64_to_sint64 255UL) in
- let b1 = sint64_to_sint8 ((Hacl.UInt64.shift_right x 48ul) @& uint64_to_sint64 255UL) in
- let b2 = sint64_to_sint8 ((Hacl.UInt64.shift_right x 40ul) @& uint64_to_sint64 255UL) in
- let b3 = sint64_to_sint8 ((Hacl.UInt64.shift_right x 32ul) @& uint64_to_sint64 255UL) in
- let b4 = sint64_to_sint8 ((Hacl.UInt64.shift_right x 24ul) @& uint64_to_sint64 255UL) in
- let b5 = sint64_to_sint8 ((Hacl.UInt64.shift_right x 16ul) @& uint64_to_sint64 255UL) in
- let b6 = sint64_to_sint8 ((Hacl.UInt64.shift_right x 8ul)  @& uint64_to_sint64 255UL) in
- let b7 = sint64_to_sint8 ((x)                              @& uint64_to_sint64 255UL) in
- upd output 0ul b0;
- upd output (1ul) b1;
- upd output (2ul) b2;
- upd output (3ul) b3;
- upd output (4ul) b4;
- upd output (5ul) b5;
- upd output (6ul) b6;
- upd output (7ul) b7
-
-let op_At_At_Amp = FStar.UInt64.logand
-
-val be_bytes_of_uint64: x:bytes -> y:u64
-  -> STL unit
-        (requires (fun h -> live h x))
-        (ensures  (fun h0 _ h1 -> live h1 x /\ modifies_1 x h0 h1))
-
-let be_bytes_of_uint64 output x =
- let b0 = uint64_to_sint8 ((FStar.UInt64.shift_right x 56ul) @@& 255UL) in
- let b1 = uint64_to_sint8 ((FStar.UInt64.shift_right x 48ul) @@& 255UL) in
- let b2 = uint64_to_sint8 ((FStar.UInt64.shift_right x 40ul) @@& 255UL) in
- let b3 = uint64_to_sint8 ((FStar.UInt64.shift_right x 32ul) @@& 255UL) in
- let b4 = uint64_to_sint8 ((FStar.UInt64.shift_right x 24ul) @@& 255UL) in
- let b5 = uint64_to_sint8 ((FStar.UInt64.shift_right x 16ul) @@& 255UL) in
- let b6 = uint64_to_sint8 ((FStar.UInt64.shift_right x 8ul)  @@& 255UL) in
- let b7 = uint64_to_sint8 ((x)                         @@& 255UL) in
- upd output 0ul b0;
- upd output (1ul) b1;
- upd output (2ul) b2;
- upd output (3ul) b3;
- upd output (4ul) b4;
- upd output (5ul) b5;
- upd output (6ul) b6;
- upd output (7ul) b7
-
-val be_uint32_of_bytes: b:bytes{length b >= 4} -> STL s32
-  (requires (fun h -> live h b))
-  (ensures (fun h0 r h1 -> h0 == h1 /\ live h0 b))
+val be_uint32_of_bytes: b:bytes{length b >= 4}
+  -> STL s32
+        (requires (fun h -> live h b))
+        (ensures (fun h0 r h1 -> h0 == h1 /\ live h0 b))
 let be_uint32_of_bytes (b:bytes{length b >= 4}) =
   let b0 = (index b 0ul) in
   let b1 = (index b 1ul) in
@@ -94,7 +144,7 @@ let rec be_uint32s_of_bytes u b len =
     be_uint32s_of_bytes u b (FStar.UInt32.sub len 4ul)
   )
 
-let op_Hat_Greater_Greater (a:s32) (b:u32) : Tot s32 = Hacl.UInt32.shift_right a b
+let op_Hat_Greater_Greater (a:s32) (b:u32) : Tot s32 = S32.shift_right a b
 
 val be_bytes_of_uint32s: output:bytes -> m:uint32s{disjoint output m} -> len:u32{v len <=length output /\ v len<=op_Multiply 4 (length m)} -> STL unit
   (requires (fun h -> live h output /\ live h m))
